1) more progress of phiplacement_bsim_wfS 2) removed redundant checks from wf_insn_base and wf_phi_operands rules 3) found a problem in the type checker    It should ensure dom-analysis must success. The current rules only use dom-analysis on-demand (when checking an instruction that needs domination property). Consider a program w/o such instructions (e.g. in the program, all blocks only contain un-conditional branches in non-entry blocks), inserting an instruction that needs dom-property is a problem, because dom-analysis can fail.
   The type-checker should run the analysis first, and stops if the
analysis fails.



git-svn-id: https://webdav.seas.upenn.edu/svn/sol/vol@3962 eef5ea85-cc2e-0410-bd84-0fae1f012da8

src3.0/Transforms/phiplacement_bsim_wfS.v
@@ -208,143 +208,173 @@ Proof.
   intros. destruct fh. inversion H. split_NoDup; auto.
 Qed.
 
-Section PresWF.
-
-Variable (los:layouts) (nts:namedts) (Ps1 Ps2:products) (pinfo:PhiInfo).
-Hypothesis (Hwfpi: WF_PhiInfo pinfo).
-
-Lemma phinodes_placement_wf_insn : forall (M M':module) (f':fdef)
-  (HeqM: M = module_intro los nts (Ps1 ++ product_fdef (PI_f pinfo) :: Ps2))
-  (HeqM': M' = module_intro los nts (Ps1 ++ product_fdef f' :: Ps2))
-  (HeqF': f' = phinodes_placement_f pinfo (PI_f pinfo)) b b' 
-  (Heqb': b' = phinodes_placement_blk pinfo b) instr
-  (HwfI : wf_insn [M] M (PI_f pinfo) b instr),
-  wf_insn [M'] M' f' b' instr.
-Proof.
-Admitted.
-
-Lemma phinodes_placement_wf_cmds : forall (M M':module) (f':fdef)
-  (HeqM: M = module_intro los nts (Ps1 ++ product_fdef (PI_f pinfo) :: Ps2))
-  (HeqM': M' = module_intro los nts (Ps1 ++ product_fdef f' :: Ps2))
-  (HeqF': f' = phinodes_placement_f pinfo (PI_f pinfo)) b b' 
-  (Heqb': b' = phinodes_placement_blk pinfo b) cs 
-  (Hwfcs : wf_cmds [M] M (PI_f pinfo) b cs),
-  wf_cmds [M'] M' f' b' cs.
-Proof.
-Admitted.
-
-Lemma phinodes_placement_wf_phinodes : forall (M M':module) (f':fdef)
-  (HeqM: M = module_intro los nts (Ps1 ++ product_fdef (PI_f pinfo) :: Ps2))
-  (HeqM': M' = module_intro los nts (Ps1 ++ product_fdef f' :: Ps2))
-  (HeqF': f' = phinodes_placement_f pinfo (PI_f pinfo)) b b' 
-  (Heqb': b' = phinodes_placement_blk pinfo b) ps
-  (Hwfps : wf_phinodes [M] M (PI_f pinfo) b ps),
-  wf_phinodes [M'] M' f' b' ps.
-Proof.
-Admitted.
-
-Lemma phinodes_placement_lookupTypViaIDFromFdef: forall (f':fdef)
-  (HeqF': f' = phinodes_placement_f pinfo (PI_f pinfo)) id0 t
-  (Hlkty: lookupTypViaIDFromFdef (PI_f pinfo) id0 = Some t),
-  lookupTypViaIDFromFdef f' id0 = Some t.
-Admitted.
-
-Lemma phinodes_placement_wf_value : forall (M M':module) (f':fdef)
-  (HeqM: M = module_intro los nts (Ps1 ++ product_fdef (PI_f pinfo) :: Ps2))
-  (HeqM': M' = module_intro los nts (Ps1 ++ product_fdef f' :: Ps2))
-  (HeqF': f' = phinodes_placement_f pinfo (PI_f pinfo)) v t
-  (Hwfv: wf_value [M] M (PI_f pinfo) v t),
-  wf_value [M'] M' f' v t.
+Lemma wf_styp__isValidElementTyp: forall S td t (Hty: wf_styp S td t),
+  isValidElementTyp t.
 Proof.
   intros.
-  inv Hwfv; try constructor.
-(*    apply insert_lookupIDFromFdef; auto. *)
-Admitted.
-
-Lemma wf_inserted: forall (M M':module) (f':fdef) 
-  (HwfF: wf_fdef [M] M (PI_f pinfo))
-  (HeqM: M = module_intro los nts (Ps1 ++ product_fdef (PI_f pinfo) :: Ps2))
-  (HeqM': M' = module_intro los nts (Ps1 ++ product_fdef f' :: Ps2))
-  (HeqF': f' = phinodes_placement_f pinfo (PI_f pinfo)) b b' 
-  (Heqb': b' = phinodes_placement_blk pinfo b)
-  (HBinF: blockInFdefB b (PI_f pinfo) = true),
-  match (PI_newids pinfo) ! (getBlockLabel b) with
-  | Some (lid, pid, sid) =>
-      match (PI_succs pinfo) ! (getBlockLabel b) with
-      | Some (_::_) =>
-          wf_insn [M'] M' f' b' 
-            (insn_cmd (insn_load lid (PI_typ pinfo) (value_id (PI_id pinfo))
-                                 (PI_align pinfo)))
-      | _ => True
-      end /\
-      match (PI_preds pinfo) ! (getBlockLabel b) with
-      | Some ((_::_) as pds) =>
-         wf_insn [M'] M' f' b' 
-           (insn_cmd (insn_store sid (PI_typ pinfo) (value_id pid)
-                        (value_id (PI_id pinfo)) (PI_align pinfo))) /\
-         wf_phinodes [M'] M' f' b' 
-            [gen_phinode pid (PI_typ pinfo) (PI_newids pinfo) pds]
-      | _ => True
-      end
-  | _ => True
-  end.
-Proof.
-  intros. 
-  assert (wf_value [M'] M' f' (value_id (PI_id pinfo)) 
-            (typ_pointer (PI_typ pinfo))) as Hwfv.
-    admit.
-  assert (wf_typ [M'] (los,nts) (PI_typ pinfo)) as Hwft.
-    admit.
-  subst.
-  remember ((PI_newids pinfo) ! (getBlockLabel b)) as R1.
-  remember ((PI_succs pinfo) ! (getBlockLabel b)) as R2.
-  remember ((PI_preds pinfo) ! (getBlockLabel b)) as R3.
-  destruct R1 as [[[lid pid] sid]|]; auto.
-  split.
-    destruct R2 as [[]|]; auto.
-    constructor; auto.
-      admit.
-
-    destruct R3 as [[]|]; auto.
-    split.
-      constructor; auto.
-        admit.
-        admit.
-
-      constructor; auto.
-        unfold gen_phinode.
-        admit.
-
-        constructor.
+  unfold isValidElementTyp, isValidElementTypB, isNotValidElementTypB.
+  inv Hty; simpl; auto.
 Qed.
 
-Lemma phinodes_placement_blockInSystemModuleFdefB: forall (M M':module) (f':fdef)
-  (HeqM: M = module_intro los nts (Ps1 ++ product_fdef (PI_f pinfo) :: Ps2))
-  (HeqM': M' = module_intro los nts (Ps1 ++ product_fdef f' :: Ps2))
-  (HeqF': f' = phinodes_placement_f pinfo (PI_f pinfo)) b b' 
-  (Heqb': b' = phinodes_placement_blk pinfo b)
-  (Hin: blockInSystemModuleFdefB b [M] M (PI_f pinfo)),
-  blockInSystemModuleFdefB b' [M'] M' f'.
-Admitted.
+Lemma getPointerAlignmentInfo_pos: forall los, 
+ (getPointerAlignmentInfo los true > 0)%nat.
+Admitted. (* Typing should check this on the top *)
 
-Ltac inv_wf_block H :=
-let S5 := fresh "S5" in
-let M5 := fresh "M5" in
-let F5 := fresh "F5" in
-let l5 := fresh "l5" in 
-let ps5 := fresh "ps5" in 
-let cs5 := fresh "cs5" in 
-let tmn5 := fresh "tmn5" in 
-let HBinSMF := fresh "HBinSMF" in 
-let Hwfps := fresh "Hwfps" in 
-let Hwfcs := fresh "Hwfcs" in 
-let Hwfi := fresh "Hwfi" in 
-let EQ1 := fresh "EQ1" in
-let EQ2 := fresh "EQ2" in
-let EQ3 := fresh "EQ3" in 
-let EQ4 := fresh "EQ4" in
-inversion H as 
-  [S5 M5 F5 l5 ps5 cs5 tmn5 HBinSMF Hwfps Hwfcs Hwfi EQ1 EQ2 EQ3 EQ4]; subst.
+Lemma wf_typ_pointer: forall S td t (Hwft: wf_typ S td t),
+  wf_typ S td (typ_pointer t).
+Proof.
+  intros. 
+  inv Hwft.
+  constructor; auto.
+    constructor; auto.
+      eapply wf_styp__isValidElementTyp; eauto.
+      apply getPointerAlignmentInfo_pos.
+Qed.
+
+Lemma WF_PhiInfo__wf_value: forall pinfo (Hwfpi : WF_PhiInfo pinfo) S M
+  (HUniq: uniqFdef (PI_f pinfo)) (HwfF : wf_fdef S M (PI_f pinfo)),
+  wf_value S M (PI_f pinfo) (value_id (PI_id pinfo)) 
+    (typ_pointer (PI_typ pinfo)).
+Proof.
+  intros.
+  destruct M.
+  constructor.
+    apply WF_PhiInfo_spec21 in HwfF; auto.
+    apply wf_typ_pointer; auto.
+
+    apply WF_PhiInfo_spec20 in HUniq; auto.
+Qed.
+
+Lemma WF_PhiInfo__lookupBlockViaIDFromFdef: forall pinfo 
+  (Hwfpi : WF_PhiInfo pinfo) (Huniq: uniqFdef (PI_f pinfo)),
+  exists b, 
+    getEntryBlock (PI_f pinfo) = Some b /\
+    lookupBlockViaIDFromFdef (PI_f pinfo) (PI_id pinfo) = Some b.
+Proof.
+  intros.
+  subst.
+  apply WF_PhiInfo_spec22 in Hwfpi; auto.
+  destruct Hwfpi as [l0 [ps0 [cs1 [cs2 [tmn0 Hentry]]]]].
+  match goal with
+  | Hentry: getEntryBlock _ = Some ?b |- _ => exists b; split; auto
+  end.
+  eapply inGetBlockIDs__lookupBlockViaIDFromFdef; eauto 1.
+    simpl. rewrite getCmdsIDs_app. simpl. xsolve_in_list.
+    solve_blockInFdefB.
+Qed.
+
+(* from dtree.v *)
+Definition getEntryLabel (f:fdef) : option l :=
+match f with
+| fdef_intro _ ((block_intro l0 _ _ _)::_) => Some l0
+| _ => None
+end.
+
+(* from dtree_props.v *)
+Lemma dom_analysis__entry_doms_others1: forall S M f 
+  (HwfF: wf_fdef S M f) entry
+  (H: getEntryLabel f = Some entry)
+  (Hex: exists b,  match (AMap.get b (dom_analyze f)) with
+                   | Dominators.mkBoundedSet dts _ => dts <> nil
+                   end),
+  (forall b, b <> entry /\ reachable f b ->
+     match (AMap.get b (dom_analyze f)) with
+     | Dominators.mkBoundedSet dts _ => In entry dts
+     end).
+Proof.
+  intros.
+  destruct H0 as [J1 J2].
+  case_eq ((dom_analyze f) !! b).
+  intros bs_contents bs_bound H1.
+  unfold dom_analyze in H1, Hex.
+  destruct f as [f b0].
+  remember (entry_dom b0) as R.
+  destruct R.
+  destruct x as [[]|]; subst.
+    destruct b0 as [|b0 b2]; inv H.
+    destruct b1; tinv y.
+    destruct bs_contents0; tinv y.
+    destruct b0 as [l1 p c t]. inv HeqR.
+    inv H2.
+    remember (
+      DomDS.fixpoint (bound_blocks (block_intro entry p c t :: b2))
+           (successors_blocks (block_intro entry p c t :: b2))
+           (transfer (bound_blocks (block_intro entry p c t :: b2)))
+           ((entry,
+            {| DomDS.L.bs_contents := nil; DomDS.L.bs_bound := bs_bound0 |})
+            :: nil)) as R.
+    destruct R.
+      symmetry in HeqR.
+      eapply EntryDomsOthers.dom_entry_doms_others with (entry:=entry) in HeqR;
+        eauto.
+        unfold EntryDomsOthers.entry_doms_others in HeqR.
+        apply HeqR in J1.
+        unfold Dominators.member in J1.
+        unfold EntryDomsOthers.dt, EntryDomsOthers.bound, DomDS.dt, DomDS.L.t
+          in J1.
+        unfold Dominators.t in H1. simpl in J1, H1.
+        rewrite H1 in J1; auto.
+
+        split.
+           remember (Kildall.successors_list
+             (EntryDomsOthers.predecessors (block_intro entry p c t :: b2))
+               entry) as R.
+           destruct R; auto.
+           assert (
+             In a
+               (Kildall.successors_list
+                 (EntryDomsOthers.predecessors (block_intro entry p c t :: b2))
+               entry)) as Hin. rewrite <- HeqR0. simpl; auto.
+           apply Kildall.make_predecessors_correct' in Hin.
+           change (successors_blocks (block_intro entry p c t :: b2)) with
+             (successors (fdef_intro f (block_intro entry p c t :: b2))) in Hin.
+           apply successors__blockInFdefB in Hin.
+           destruct Hin as [ps0 [cs0 [tmn0 [G1 G2]]]].
+           eapply getEntryBlock_inv with (l3:=a)(a:=entry) in G2; simpl; eauto.
+           congruence.
+
+        split; auto.
+          exists{| DomDS.L.bs_contents := nil; DomDS.L.bs_bound := bs_bound0 |}.
+          simpl.
+          split; auto.
+            split; intros x Hin; auto.
+
+      rewrite AMap.gso in H1; auto.
+      rewrite AMap.gi in H1. inv H1.
+      destruct Hex as [b0 Hex].
+      destruct (l_dec entry b0); subst.
+        rewrite AMap.gss in Hex; auto. congruence.
+
+        rewrite AMap.gso in Hex; auto. rewrite AMap.gi in Hex. simpl in Hex.
+        contradict Hex; auto.
+
+    inv H.
+Qed.
+
+Lemma entry_blockStrictDominates_others: forall s m f (HwfF : wf_fdef s m f)
+  (b be : block) (Hentry : getEntryBlock f = ret be)
+  (n : getBlockLabel be <> getBlockLabel b)
+  (Hreach : isReachableFromEntry f b),
+  blockStrictDominates f be b.
+Proof.
+  unfold blockStrictDominates.
+  intros.
+  destruct be as [l1 ? ? ?].
+  destruct b as [l2 ? ? ?].
+  simpl in n.
+  assert (getEntryLabel f = Some l1) as Gentry.
+    destruct f as [? blocks5].
+    destruct blocks5; inv Hentry. auto.
+  eapply dom_analysis__entry_doms_others1 with (b:=l2) in Gentry; eauto.
+    admit. (* typings should ensure dom_analysis always succeeds. *)
+Qed.
+
+Lemma isReachableFromEntry_dec: forall f b,
+  isReachableFromEntry f b \/ ~ isReachableFromEntry f b.
+Proof.
+  destruct f as [fh bs]. destruct b as [l0 ? ? ?]. simpl.
+  apply reachable_dec; auto.
+Qed.
 
 Lemma wf_cmds_intro: forall s m f b cs,
   (forall c, In c cs -> wf_insn s m f b (insn_cmd c)) ->
@@ -382,11 +412,1186 @@ Proof.
     inv Hwfps1. constructor; auto.
 Qed.
 
-Lemma phinodes_placement_wf_block : forall (M M':module) (f':fdef)
-  (HwfF: wf_fdef [M] M (PI_f pinfo))
-  (HeqM: M = module_intro los nts (Ps1 ++ product_fdef (PI_f pinfo) :: Ps2))
-  (HeqM': M' = module_intro los nts (Ps1 ++ product_fdef f' :: Ps2))
-  (HeqF': f' = phinodes_placement_f pinfo (PI_f pinfo)) b
+Ltac inv_wf_block H :=
+let S5 := fresh "S5" in
+let M5 := fresh "M5" in
+let F5 := fresh "F5" in
+let l5 := fresh "l5" in 
+let ps5 := fresh "ps5" in 
+let cs5 := fresh "cs5" in 
+let tmn5 := fresh "tmn5" in 
+let HBinSMF := fresh "HBinSMF" in 
+let Hwfps := fresh "Hwfps" in 
+let Hwfcs := fresh "Hwfcs" in 
+let Hwfi := fresh "Hwfi" in 
+let EQ1 := fresh "EQ1" in
+let EQ2 := fresh "EQ2" in
+let EQ3 := fresh "EQ3" in 
+let EQ4 := fresh "EQ4" in
+inversion H as 
+  [S5 M5 F5 l5 ps5 cs5 tmn5 HBinSMF Hwfps Hwfcs Hwfi EQ1 EQ2 EQ3 EQ4];
+subst S5 M5 F5.
+
+Ltac inv_wf_fdef H :=
+let S5 := fresh "S5" in
+let los5 := fresh "los5" in
+let nts5 := fresh "nts5" in
+let prods5 := fresh "prods5" in
+let fh5 := fresh "fh5" in
+let bs5 := fresh "bs5" in
+let b5 := fresh "b5" in
+let udb5 := fresh "udb5" in
+let HpInS := fresh "HpInS" in
+let Hwffh := fresh "Hwffh" in
+let Hentry := fresh "Hentry" in
+let EQ0 := fresh "EQ0" in
+let Hnpred := fresh "Hnpred" in
+let Hwfb := fresh "Hwfb" in
+let EQ1 := fresh "EQ1" in
+let EQ2 := fresh "EQ2" in
+let EQ3 := fresh "EQ3" in
+inversion H as 
+  [S5 los5 nts5 prods5 fh5 bs5 b5 udb5 HpInS Hwffh Hentry EQ0 Hnpred
+   Hwfb EQ1 EQ2 EQ3]; subst udb5 S5.
+
+Lemma In_InBlocksB: forall b bs, In b bs -> InBlocksB b bs = true.
+Admitted.
+
+(* entry_cmds_simulation in phiplacement_bsim_defs.v should 
+   also use the lemma *)
+Lemma PI_preds_of_entry_cannot_be_nonempty: forall s m pinfo
+  (HwfF: wf_fdef s m (PI_f pinfo)) b
+  (Hentry: getEntryBlock (PI_f pinfo) = Some b),
+  forall (pd : l) (pds : list l), 
+    (PI_preds pinfo) ! (getBlockLabel b) <> ret (pd :: pds).
+Proof.
+  intros.
+  unfold PI_preds.
+  intros. intro J.
+  assert (In pd (make_predecessors (PI_succs pinfo))!!!(getBlockLabel b)) as G.
+    unfold successors_list. unfold l in J. rewrite J. simpl. auto.
+  apply make_predecessors_correct' in G.
+  unfold PI_succs in G.
+  apply successors__blockInFdefB in G.
+  destruct G as [ps1 [cs1' [tmn1 [G1 G2]]]].
+  destruct (PI_f pinfo) as [fh bs].
+  simpl in G1.
+  destruct b.
+  eapply getEntryBlock_inv in G1; eauto.
+Qed.
+
+(* wf_phi_operands doesnt depend on i0 and t0, which should be removed. *)
+Lemma wf_phi_operands__intro : forall f b i0 t0 vls0,
+  (forall vid1 l1 (Hin: In (value_id vid1, l1) vls0), 
+     exists b1,
+      lookupBlockViaLabelFromFdef f l1 = Some b1 /\
+      ((exists vb,
+         lookupBlockViaIDFromFdef f vid1 = Some vb /\
+         (blockDominates f vb b1 \/ not (isReachableFromEntry f b))) \/
+      In vid1 (getArgsIDsOfFdef f))) ->
+  wf_phi_operands f b i0 t0 vls0.
+Proof.
+  induction vls0 as [|[[vid5|] l0]]; intros.
+    constructor.
+
+    assert (In (value_id vid5, l0) ((value_id vid5, l0) :: vls0)) as Hin.
+      xsolve_in_list.
+    apply H in Hin.
+    destruct Hin as [b1 [J1 J2]].
+    econstructor; eauto.
+      apply IHvls0.
+      intros.
+      apply H. simpl. auto.
+
+    constructor.
+      apply IHvls0.
+      intros.
+      apply H. simpl. auto.
+Qed.
+
+Lemma wf_phi_operands__elim' : forall f b i0 t0 vls0 vid1 l1
+  (Hwfop: wf_phi_operands f b i0 t0 vls0)
+  (Hin: In (value_id vid1, l1) vls0),
+  exists b1,
+    lookupBlockViaLabelFromFdef f l1 = Some b1 /\
+    ((exists vb,
+       lookupBlockViaIDFromFdef f vid1 = Some vb /\
+       (blockDominates f vb b1 \/ not (isReachableFromEntry f b))) \/
+    In vid1 (getArgsIDsOfFdef f)).
+Proof.
+  induction 1; intros.
+    tauto.
+
+    destruct_in Hin.
+      inv Hin. eauto.
+
+    destruct_in Hin.
+      congruence.
+Qed.
+
+(* from dtree_props.v *)
+Lemma In_bound_fdef__blockInFdefB: forall f l3,
+  In l3 (bound_fdef f) ->
+  exists ps, exists cs, exists tmn,
+    blockInFdefB (block_intro l3 ps cs tmn) f = true.
+Admitted. (* infra *)
+
+Lemma PI_newids_are_in_PI_rd: forall pinfo l1 (Huniq: uniqFdef (PI_f pinfo)),
+  WF_PhiInfo pinfo ->
+  (PI_newids pinfo) ! l1 <> merror ->
+  In l1 (PI_rd pinfo).
+Proof.
+  intros.
+Admitted.
+
+Lemma PI_rd__lookupBlockViaLabelFromFdef: forall pinfo (Hwfpi: WF_PhiInfo pinfo) l0,
+  In l0 (PI_rd pinfo) ->
+  exists b1 : block,
+    lookupBlockViaLabelFromFdef (PI_f pinfo) l0 = ret b1 /\
+    isReachableFromEntry (PI_f pinfo) b1.
+Admitted.
+
+Lemma blockDominates_refl: forall f b, blockDominates f b b.
+Proof.
+  unfold blockDominates.
+  destruct b. destruct (dom_analyze f) !! l5. auto.
+Qed.
+
+Lemma WF_PhiInfo_br_preds_succs: forall pinfo l0 l3 (Hwfpi : WF_PhiInfo pinfo)
+  prds (Hin : In l3 prds) (Heq' : (PI_preds pinfo) ! l0 = ret prds),
+  exists succs, (PI_succs pinfo) ! l3 = ret succs /\ In l0 succs.
+Proof.
+  unfold PI_preds. unfold PI_succs.
+  intros.
+  destruct Hwfpi as [J1 J2].
+  assert (In l3 ((make_predecessors (successors (PI_f pinfo)))!!!l0)) as Hin'.
+    unfold successors_list.
+    unfold ls, l in *.
+    rewrite Heq'. auto.
+  apply make_predecessors_correct' in Hin'.
+  unfold successors_list in Hin'.
+  remember (@ATree.get (list atom) l3 (successors (PI_f pinfo))) as R.
+  destruct R; tinv Hin'. eauto.
+Qed.
+
+Lemma InPhiNodes_lookupTypViaIDFromPhiNodes' : forall ps p,
+  NoDup (getPhiNodesIDs ps) ->
+  In p ps ->
+  lookupTypViaIDFromPhiNodes ps (getPhiNodeID p) = Some (getPhiNodeTyp p).
+Proof.
+  induction ps; intros.
+    inversion H0.
+
+    simpl in *.
+    inv H. unfold lookupTypViaIDFromPhiNodes, lookupTypViaIDFromPhiNode.
+    destruct H0 as [H0 | H0]; subst.
+      destruct (@eq_dec id 
+        (@EqDec_eq_of_EqDec id EqDec_atom) (getPhiNodeID p) (getPhiNodeID p)); 
+        subst; auto.
+        congruence.
+
+      destruct (@eq_dec id 
+        (@EqDec_eq_of_EqDec id EqDec_atom) (getPhiNodeID p) (getPhiNodeID a)); 
+        subst; auto.
+
+        contradict H3; auto.
+        rewrite <- e. solve_in_list.
+Qed.
+
+Lemma uniqF__lookupPhiNodeTypViaIDFromFdef : forall l1 ps1 cs1 tmn1 f p,
+  uniqFdef f ->
+  blockInFdefB (block_intro l1 ps1 cs1 tmn1) f = true ->
+  In p ps1 ->
+  lookupTypViaIDFromFdef f (getPhiNodeID p) = Some (getPhiNodeTyp p).
+Proof.
+  intros.
+  destruct f as [f b].
+  destruct f as [fnattrs5 typ5 id5 args5 varg5]. inversion H.
+  split_NoDup.
+  simpl in *.
+  assert (In (getPhiNodeID p) (getBlocksLocs b)) as Hin.
+    eapply in_getBlockLocs__in_getBlocksLocs in H0; eauto.
+    simpl. xsolve_in_list.
+  destruct H as [J1 J2].
+  assert (~ In (getPhiNodeID p) (getArgsIDs args5)) as Hnotin.
+    eapply NoDup_disjoint; eauto.
+  apply NotInArgsIDs_lookupTypViaIDFromArgs in Hnotin.
+  rewrite Hnotin.
+  eapply lookupTypViaIDFromBlock__inBlocks; eauto.
+  simpl.
+  apply NoDup__InBlocksB in H0; auto.
+  simpl in H0.
+  split_NoDup.
+  rewrite InPhiNodes_lookupTypViaIDFromPhiNodes'; auto.
+Qed.
+
+Lemma phinodes_placement_blk_tail_inv: forall pinfo b lid pid sid scs
+  (HeqR1 : ret (lid, pid, sid) = (PI_newids pinfo) ! (getBlockLabel b))
+  (HeqR2 : ret scs = (PI_succs pinfo) ! (getBlockLabel b))
+  (Hnonempty: scs <> nil),
+  exists l0, exists ps0, exists cs0, exists tmn0, exists ps1, exists cs1,
+    b = block_intro l0 ps0 cs0 tmn0 /\
+    phinodes_placement_blk pinfo b = 
+      block_intro l0 (ps1++ps0)
+        (cs1 ++ cs0 ++ 
+         [insn_load lid (PI_typ pinfo) (value_id (PI_id pinfo))
+           (PI_align pinfo)]) tmn0.
+Proof.
+  intros. destruct b as [l0 ps0 cs0 tmn0]. simpl in *. 
+  exists l0. exists ps0. exists cs0. exists tmn0.
+  rewrite <- HeqR1. rewrite <- HeqR2. 
+  destruct scs; try congruence.
+  destruct ((PI_preds pinfo) ! l0) as [[]|].
+    exists nil. exists nil. auto.
+
+    match goal with
+    | |- context [ block_intro _ (?p::_) (?c::_++_) _] => 
+         exists [p]; exists [c]; simpl_env; auto
+    end.
+ 
+    exists nil. exists nil. auto.
+Qed.
+
+Lemma phinodes_placement_blk_head_inv: forall pinfo b lid pid sid pds
+  (HeqR1 : ret (lid, pid, sid) = (PI_newids pinfo) ! (getBlockLabel b))
+  (HeqR3 : ret pds = (PI_preds pinfo) ! (getBlockLabel b))
+  (Hneq : pds <> nil),
+  exists l0, exists ps0, exists cs0, exists tmn0, exists cs2,
+    b = block_intro l0 ps0 cs0 tmn0 /\
+    phinodes_placement_blk pinfo b = 
+      block_intro l0 
+        ([gen_phinode pid (PI_typ pinfo) (PI_newids pinfo) pds]++ps0)
+        ([insn_store sid (PI_typ pinfo) (value_id pid)
+           (value_id (PI_id pinfo)) (PI_align pinfo)] ++ cs0 ++ cs2) tmn0.
+Proof.
+  intros. destruct b as [l0 ps0 cs0 tmn0]. simpl in *. 
+  exists l0. exists ps0. exists cs0. exists tmn0.
+  rewrite <- HeqR1. rewrite <- HeqR3. 
+  destruct pds; try congruence.
+  destruct ((PI_succs pinfo) ! l0) as [[]|].
+    exists nil. auto.
+
+    match goal with
+    | |- context [ (_::_++[?c]) ] => exists [c]; simpl_env; auto
+    end.
+
+    exists nil. auto.
+Qed.
+
+Lemma phinodes_placement_blk_inv: forall pinfo b,
+  exists l0, exists ps0, exists cs0, exists tmn0, 
+    exists ps1, exists cs1, exists cs2,
+    b = block_intro l0 ps0 cs0 tmn0 /\
+    phinodes_placement_blk pinfo b = 
+      block_intro l0 (ps1++ps0) (cs1 ++ cs0 ++ cs2) tmn0.
+Proof.
+  intros. destruct b as [l0 ps0 cs0 tmn0]. simpl in *. 
+  exists l0. exists ps0. exists cs0. exists tmn0.
+  destruct ((PI_newids pinfo) ! l0) as [[[]]|].
+    destruct ((PI_preds pinfo) ! l0) as [[]|]; try solve [
+      exists nil; exists nil;
+      destruct ((PI_succs pinfo) ! l0) as [[]|]; try solve [
+        exists nil; auto |
+        match goal with
+        | |- context [ (_++[?c]) ] => exists [c]; simpl_env; auto
+        end
+      ] |
+
+      match goal with
+      | |- context [ block_intro _ (?p::_) (?c::_++_) _] => 
+           exists [p]; exists [c]
+      end;
+      destruct ((PI_succs pinfo) ! l0) as [[]|]; try solve [
+        exists nil; auto |
+        match goal with
+        | |- context [ (_::_++[?c]) ] => exists [c]; simpl_env; auto
+        end
+      ]
+    ].
+
+    exists nil. exists nil. exists nil. simpl_env. auto.
+Qed.
+
+Ltac solve_refl :=
+match goal with
+| |- ?c =cmd= ?c = true => apply cmdEqB_refl
+| |- ?p =phi= ?p = true => apply phinodeEqB_refl
+| |- moduleEqB ?m ?m = true => apply moduleEqB_refl
+end.
+
+Section PresWF.
+
+Variable (los:layouts) (nts:namedts) (Ps1 Ps2:products) (pinfo:PhiInfo)
+         (M M':module) (f':fdef).
+Hypothesis (Hwfpi: WF_PhiInfo pinfo)   
+           (HeqM: M = module_intro los nts (Ps1 ++ product_fdef (PI_f pinfo) :: Ps2))
+           (HeqM': M' = module_intro los nts (Ps1 ++ product_fdef f' :: Ps2))
+           (HeqF': f' = phinodes_placement_f pinfo (PI_f pinfo))
+           (HwfF: wf_fdef [M] M (PI_f pinfo)) 
+           (HuniqF: uniqFdef (PI_f pinfo)).
+
+Lemma phinodes_placement_lookupTypViaIDFromFdef: forall id0 t
+  (Hlkty: lookupTypViaIDFromFdef (PI_f pinfo) id0 = Some t),
+  lookupTypViaIDFromFdef f' id0 = Some t.
+Admitted.
+
+Lemma phinodes_placement_wf_const : forall c t
+  (Hwfc: wf_const [M] (los,nts) c t),
+  wf_const [M'] (los,nts) c t.
+
+Admitted.
+
+Lemma phinodes_placement_wf_value : forall v t
+  (Hwfv: wf_value [M] M (PI_f pinfo) v t),
+  wf_value [M'] M' f' v t.
+Proof.
+  intros.
+  assert (J1:=phinodes_placement_wf_const).
+  assert (J2:=phinodes_placement_lookupTypViaIDFromFdef).
+  inv Hwfv; uniq_result;
+    constructor; eauto using wf_typ_independent.
+Qed.
+
+Lemma phinodes_placement_insnInFdefBlockB: forall b instr,
+  insnInFdefBlockB instr (PI_f pinfo) b = true ->
+  insnInFdefBlockB instr (phinodes_placement_f pinfo (PI_f pinfo))
+    (phinodes_placement_blk pinfo b) = true.
+Admitted.
+
+Lemma phinodes_placement_insnDominates: forall b b' instr
+  (Hin: insnInFdefBlockB instr (PI_f pinfo) b = true)
+  (Heqb': b' = phinodes_placement_blk pinfo b) id_
+  (Hdom: insnDominates id_ instr b),
+  insnDominates id_ instr b'.
+Proof.
+  unfold insnDominates.
+  intros. subst.
+  assert (J:=phinodes_placement_blk_inv pinfo b).
+  destruct J as [l0 [ps0 [cs0 [tmn0 [ps1 [cs1 [cs2 [EQ J]]]]]]]]; subst.
+  rewrite J. 
+  destruct instr; auto.
+    destruct Hdom as [[ps1' [p1 [ps2 [J1 J2]]]] | 
+                      [cs1' [c1 [cs2' [cs3 [J1 J2]]]]]]; subst.
+      left. exists (ps1++ps1'). exists p1. exists ps2. simpl_env. auto.
+      right. exists (cs1++cs1'). exists c1. exists cs2'. exists (cs3++cs2).
+        simpl_env. auto.
+    destruct Hdom as [Hdom EQ]; subst.
+    split; auto.
+    destruct Hdom as [[cs1' [c1 [cs2' [J1 J2]]]] |
+                      [ps1' [p1 [ps2 [J1 J2]]]]]; subst.
+      left. exists (cs1++cs1'). exists c1. exists (cs2'++cs2).
+        simpl_env. auto.
+      right. exists (ps1++ps1'). exists p1. exists ps2. simpl_env. auto.
+Qed.
+
+Lemma phinodes_placemen_getArgsIDsOfFdef:
+  getArgsIDsOfFdef (PI_f pinfo) =
+    getArgsIDsOfFdef (phinodes_placement_f pinfo (PI_f pinfo)).
+Admitted.
+
+Lemma phinodes_placement_lookupBlockViaIDFromFdef: forall id0 b,
+  lookupBlockViaIDFromFdef (PI_f pinfo) id0 = Some b ->
+  lookupBlockViaIDFromFdef (phinodes_placement_f pinfo (PI_f pinfo)) id0 
+    = Some (phinodes_placement_blk pinfo b).
+Admitted.
+
+Lemma phinodes_placement_wf_operand: forall b b'
+  (Heqb': b' = phinodes_placement_blk pinfo b) instr id_
+  (Hwfop: wf_operand (PI_f pinfo) b instr id_),
+  wf_operand f' b' instr id_.
+Proof.
+  intros.
+  inv Hwfop.
+  assert (J:=H). 
+  apply phinodes_placement_insnInFdefBlockB in H.
+  econstructor; eauto 1.  
+    rewrite <- phinodes_placemen_getArgsIDsOfFdef.
+    destruct H3 as [[b0 [J1 H3]] | J3]; auto.
+    left.
+    exists (phinodes_placement_blk pinfo b0).
+    split.
+      apply phinodes_placement_lookupBlockViaIDFromFdef; auto.
+
+      fold_PhiPlacement_tac.
+      rewrite <- TransCFG.pres_blockStrictDominates; auto.
+      rewrite <- TransCFG.pres_isReachableFromEntry; auto.
+      destruct H3 as [H3 | [H3 | H3]]; auto.
+      left.
+      eapply phinodes_placement_insnDominates; eauto.
+Qed.
+
+Lemma phinodes_placement_wf_insn_base: forall b b'
+  (Heqb': b' = phinodes_placement_blk pinfo b) instr
+  (HwfI: wf_insn_base (PI_f pinfo) b instr),
+  wf_insn_base f' b' instr.
+Proof.
+  intros.
+  assert (J:=@phinodes_placement_wf_operand b b' Heqb' instr).
+  inv HwfI.
+  apply phinodes_placement_insnInFdefBlockB in H.
+  econstructor; eauto 1.
+    intros id_ Hin.
+    apply H2 in Hin. auto.
+Qed.
+
+Lemma phinodes_placement_getDefReturnType:
+  Function.getDefReturnType (phinodes_placement_f pinfo (PI_f pinfo)) =
+  Function.getDefReturnType (PI_f pinfo).
+Proof.
+  assert (fheaderOfFdef (PI_f pinfo) = 
+          fheaderOfFdef (phinodes_placement_f pinfo (PI_f pinfo))) as EQ.
+    rewrite <- phinodes_placement_f_spec1.
+    apply phinodes_placement_fheaderOfFdef.
+  unfold Function.getDefReturnType.
+  destruct (phinodes_placement_f pinfo (PI_f pinfo)) as [[]].
+  destruct (PI_f pinfo) as [[]].
+  inv EQ. auto.
+Qed.
+
+Lemma phinodes_placement_lookupBlockViaLabelFromFdef: forall l0 b,
+  lookupBlockViaLabelFromFdef (PI_f pinfo) l0 = Some b ->
+  lookupBlockViaLabelFromFdef (phinodes_placement_f pinfo (PI_f pinfo)) l0 
+    = Some (phinodes_placement_blk pinfo b).
+Admitted.
+
+Lemma phinodes_placement_wf_trunc : forall b b' 
+  (Heqb': b' = phinodes_placement_blk pinfo b) instr
+  (HwfI : wf_trunc [M] M (PI_f pinfo) b instr),
+  wf_trunc [M'] M' f' b' instr.
+Proof.
+  intros.
+  assert (J1:=@phinodes_placement_wf_insn_base b b' Heqb' instr).
+  assert (J2:=phinodes_placement_wf_value).
+  assert (J3:=@wf_typ_independent [M] [M'] (los,nts)).
+  inv HwfI; uniq_result; try solve [
+    econstructor; eauto 3
+  ].
+Qed.
+
+Lemma phinodes_placement_wf_ext : forall b b' 
+  (Heqb': b' = phinodes_placement_blk pinfo b) instr
+  (HwfI : wf_ext [M] M (PI_f pinfo) b instr),
+  wf_ext [M'] M' f' b' instr.
+Proof.
+  intros.
+  assert (J1:=@phinodes_placement_wf_insn_base b b' Heqb' instr).
+  assert (J2:=phinodes_placement_wf_value).
+  assert (J3:=@wf_typ_independent [M] [M'] (los,nts)).
+  inv HwfI; uniq_result; try solve [
+    econstructor; eauto 3
+  ].
+Qed.
+
+Lemma phinodes_placement_wf_cast : forall b b' 
+  (Heqb': b' = phinodes_placement_blk pinfo b) instr
+  (HwfI : wf_cast [M] M (PI_f pinfo) b instr),
+  wf_cast [M'] M' f' b' instr.
+Proof.
+  intros.
+  assert (J1:=@phinodes_placement_wf_insn_base b b' Heqb' instr).
+  assert (J2:=phinodes_placement_wf_value).
+  assert (J3:=@wf_typ_independent [M] [M'] (los,nts)).
+  inv HwfI; uniq_result; try solve [
+    econstructor; eauto 3
+  ].
+Qed.
+
+Lemma phinodes_placement_wf_phi_operands : forall b b' 
+  (Heqb': b' = phinodes_placement_blk pinfo b) id0 t0 vls0
+  (Hwfps: wf_phi_operands (PI_f pinfo) b id0 t0 vls0),
+  wf_phi_operands f' b' id0 t0 vls0.
+Proof.
+  intros. subst.
+  apply wf_phi_operands__intro.
+  intros.
+  eapply wf_phi_operands__elim' in Hwfps; eauto.
+  rewrite <- phinodes_placemen_getArgsIDsOfFdef.
+  destruct Hwfps as [b1 [J1 Hwfps]].
+  exists (phinodes_placement_blk pinfo b1).
+  split.
+    apply phinodes_placement_lookupBlockViaLabelFromFdef; auto.
+
+    destruct Hwfps as [[b0 [J2 Hwfps]] | J3]; auto.
+    left.
+    exists (phinodes_placement_blk pinfo b0).
+    split.
+      apply phinodes_placement_lookupBlockViaIDFromFdef; auto.
+
+      fold_PhiPlacement_tac.
+      rewrite <- TransCFG.pres_blockDominates; auto.
+      rewrite <- TransCFG.pres_isReachableFromEntry; auto.
+Qed.
+
+Lemma phinodes_placement_check_list_value_l : forall b b' 
+  (Heqb': b' = phinodes_placement_blk pinfo b) vls0
+  (hwfps: check_list_value_l (PI_f pinfo) b vls0),
+  check_list_value_l f' b' vls0.
+Proof.
+  unfold check_list_value_l.
+  intros. destruct_let. subst.
+  fold_PhiPlacement_tac.
+  rewrite <- TransCFG.pres_genBlockUseDef_fdef; auto.
+  rewrite <- TransCFG.pres_predOfBlock; auto.
+Qed.
+
+Lemma phinodes_placement_wf_phinode : forall b b' 
+  (Heqb': b' = phinodes_placement_blk pinfo b) pnode
+  (HwfI : wf_phinode (PI_f pinfo) b pnode),
+  wf_phinode f' b' pnode.
+Proof.
+  unfold wf_phinode.
+  intros.
+  destruct pnode as [id0 t0 vls0].
+  destruct HwfI as [J1 J2].
+  eapply phinodes_placement_wf_phi_operands in J1; eauto.
+  eapply phinodes_placement_check_list_value_l in J2; eauto.
+Qed.
+
+Lemma phinodes_placement_wf_insn : forall b b' 
+  (Heqb': b' = phinodes_placement_blk pinfo b) instr
+  (HwfI : wf_insn [M] M (PI_f pinfo) b instr),
+  wf_insn [M'] M' f' b' instr.
+Proof.
+  intros.
+  assert (J1:=@phinodes_placement_wf_insn_base b b' Heqb' instr).
+  assert (J2:=phinodes_placement_wf_value).
+  assert (J3:=@wf_typ_independent [M] [M'] (los,nts)).
+  assert (J4:=phinodes_placement_wf_const).
+  assert (J5:=@phinodes_placement_wf_trunc b b' Heqb' instr).
+  assert (J6:=@phinodes_placement_wf_ext b b' Heqb' instr).
+  assert (J7:=@phinodes_placement_wf_cast b b' Heqb' instr).
+  assert (J8:=@phinodes_placement_wf_phinode b b' Heqb').
+
+Ltac phinodes_placement_wf_insn_tac :=
+repeat match goal with
+| H1 : lookupBlockViaLabelFromFdef (PI_f pinfo) _ = ret _ |- _ =>
+  apply phinodes_placement_lookupBlockViaLabelFromFdef in H1
+| H1 : context [Function.getDefReturnType (PI_f pinfo)] |- _ =>
+  rewrite <- phinodes_placement_getDefReturnType in H1
+| |- context [Function.getDefReturnType (PI_f pinfo)] =>
+  rewrite <- phinodes_placement_getDefReturnType
+| H1 : insnInFdefBlockB _ (PI_f pinfo) _ = true |- _ =>
+  apply phinodes_placement_insnInFdefBlockB in H1
+end.
+
+  inv HwfI; uniq_result; try solve [
+    phinodes_placement_wf_insn_tac;
+    econstructor; eauto 3
+  ].
+Qed.
+
+Lemma phinodes_placement_wf_cmds : forall b b' 
+  (Heqb': b' = phinodes_placement_blk pinfo b) cs 
+  (Hwfcs : wf_cmds [M] M (PI_f pinfo) b cs),
+  wf_cmds [M'] M' f' b' cs.
+Proof.
+  intros.
+  induction cs; intros.
+    constructor.
+
+    inversion Hwfcs.
+    econstructor; eauto using phinodes_placement_wf_insn.
+Qed.
+
+Lemma phinodes_placement_wf_phinodes : forall b b' 
+  (Heqb': b' = phinodes_placement_blk pinfo b) ps
+  (Hwfps : wf_phinodes [M] M (PI_f pinfo) b ps),
+  wf_phinodes [M'] M' f' b' ps.
+Proof.
+  intros.
+  induction ps; intros.
+    constructor.
+
+    inversion Hwfps.
+    econstructor; eauto using phinodes_placement_wf_insn.
+Qed.
+
+Lemma inserted_load__in__phinodes_placement_blk: forall b lid pid sid scs
+  (HeqR1 : ret (lid, pid, sid) = (PI_newids pinfo) ! (getBlockLabel b))
+  (HeqR2 : ret scs = (PI_succs pinfo) ! (getBlockLabel b))
+  (Hnonempty: scs <> nil) (Hin: blockInFdefB b (PI_f pinfo) = true),
+  insnInFdefBlockB
+     (insn_cmd
+        (insn_load lid (PI_typ pinfo) (value_id (PI_id pinfo))
+           (PI_align pinfo))) (phinodes_placement_f pinfo (PI_f pinfo))
+     (phinodes_placement_blk pinfo b) = true.
+Proof.
+  intros.
+  eapply phinodes_placement_blk_tail_inv in HeqR1; eauto 1.
+  destruct HeqR1 as [l0 [ps0 [cs0 [tmn0 [ps1 [cs1 [EQ1 EQ2]]]]]]]; subst.
+  apply insnInFdefBlockB_intro.
+    rewrite EQ2.
+    simpl. apply In_InCmdsB. xsolve_in_list.
+  
+    fold_PhiPlacement_tac.
+    apply TransCFG.pres_blockInFdefB; auto.
+Qed.
+
+Ltac solve_isNotPhiNode := unfold isPhiNode; simpl; congruence.
+
+Lemma phinodes_placement_blk_rev_eq: forall (pinfo : PhiInfo) (b : block)
+  (Huniq : uniqFdef (PI_f pinfo))
+  (Hin : blockInFdefB b (PI_f pinfo) = true) (be : block)
+  (Hentry : getEntryBlock (PI_f pinfo) = ret be)
+  (e : getBlockLabel (phinodes_placement_blk pinfo be) =
+       getBlockLabel (phinodes_placement_blk pinfo b)),
+  be = b.
+Proof.
+  intros.
+  rewrite <- phinodes_placement_blk__getBlockLabel in e.
+  rewrite <- phinodes_placement_blk__getBlockLabel in e.
+  apply entryBlockInFdef in Hentry.
+  destruct b. destruct be.        
+  simpl in e. subst l0.
+  eapply blockInFdefB_uniq in Hin; eauto.
+  f_equal; tauto.
+Qed.
+
+Lemma wf_operand_pid__in__inserted_load: forall b lid pid sid scs
+  (HeqR1 : ret (lid, pid, sid) = (PI_newids pinfo) ! (getBlockLabel b))
+  (HeqR2 : ret scs = (PI_succs pinfo) ! (getBlockLabel b))
+  (Hnonempty: scs <> nil) (Huniq: uniqFdef (PI_f pinfo))
+  (Hin: blockInFdefB b (PI_f pinfo) = true),
+  wf_operand (phinodes_placement_f pinfo (PI_f pinfo))
+     (phinodes_placement_blk pinfo b)
+     (insn_cmd
+        (insn_load lid (PI_typ pinfo) (value_id (PI_id pinfo))
+           (PI_align pinfo))) (PI_id pinfo).
+Proof.
+  intros.
+  econstructor; simpl; eauto 2; simpl; auto.
+    eapply inserted_load__in__phinodes_placement_blk; eauto.
+    solve_isNotPhiNode.
+
+    left. assert (J:=Hwfpi).
+    apply WF_PhiInfo__lookupBlockViaIDFromFdef in J; auto.
+    destruct J as [be [Hentry Hlkup]]. 
+    apply phinodes_placement_lookupBlockViaIDFromFdef in Hlkup.
+    exists (phinodes_placement_blk pinfo be).
+    split; auto.
+    destruct (isReachableFromEntry_dec
+                (phinodes_placement_f pinfo (PI_f pinfo))
+                (phinodes_placement_blk pinfo b)); auto.
+    destruct (eq_atom_dec (getBlockLabel (phinodes_placement_blk pinfo be))
+                          (getBlockLabel (phinodes_placement_blk pinfo b))).
+    Case "be = b".
+      left.
+      assert (be = b) as EQ.
+        eapply phinodes_placement_blk_rev_eq; eauto.
+      subst.
+      assert (J:=Hwfpi).
+      apply WF_PhiInfo_spec22 in J; auto.
+      destruct J as [l0 [ps0 [cs1 [cs3 [tmn0 Hentry']]]]].
+      uniq_result.
+      eapply phinodes_placement_blk_tail_inv in HeqR1; eauto 1.
+      destruct HeqR1 as [l1 [ps1 [cs4 [tmn1 [ps5 [cs5 [EQ1 EQ2]]]]]]].
+      uniq_result.
+      rewrite EQ2. clear EQ2.
+      simpl. right.
+      simpl_env.
+      match goal with
+      | |- context [?A ++ ?B ++ [?c] ++ ?D ++ [?e] = _ ] =>
+        exists (A++B); exists c; exists D; exists nil; simpl_env; split; auto
+      end.
+
+    Case "be <> b".
+      right. left.
+      fold_PhiPlacement_tac.
+      erewrite <- TransCFG.pres_blockStrictDominates; eauto.
+      assert (isReachableFromEntry (PI_f pinfo) b) as Hreach.
+        erewrite (@TransCFG.pres_isReachableFromEntry (PhiPlacement pinfo)); 
+          eauto.
+      rewrite <- phinodes_placement_blk__getBlockLabel in n.
+      rewrite <- phinodes_placement_blk__getBlockLabel in n.
+      eapply entry_blockStrictDominates_others; eauto.
+Qed.
+
+Lemma wf_PI_typ': wf_typ [M'] (los, nts) (PI_typ pinfo).
+Proof.
+  subst.
+  apply WF_PhiInfo_spec21 in HwfF; auto.
+  eapply wf_typ_independent; eauto.
+Qed.
+
+Lemma WF_PhiInfo_br_preds_succs': forall (pinfo : PhiInfo) 
+  (Hwfpi : WF_PhiInfo pinfo) (HuniqF : uniqFdef (PI_f pinfo)) (pds : list l)
+  (b : block) (HeqR3 : ret pds = (PI_preds pinfo) ! (getBlockLabel b))
+  (l0 : l) (Hin : In l0 pds) (b1 : block)
+  (Hlkup : lookupBlockViaLabelFromFdef (PI_f pinfo) l0 = ret b1),
+  l0 = getBlockLabel b1 /\
+  exists succs,
+    succs <> nil /\ ret succs = (PI_succs pinfo) ! (getBlockLabel b1).
+Proof.
+  intros.
+  symmetry in HeqR3.
+  eapply WF_PhiInfo_br_preds_succs in HeqR3; eauto.
+  destruct HeqR3 as [succs [J1 J2]].
+  assert (succs <> nil) as Hneq'.
+    destruct succs; tinv J2. congruence.
+  symmetry in J1.
+  assert (l0 = getBlockLabel b1) as EQ.
+    destruct b1.
+    apply lookupBlockViaLabelFromFdef_inv in Hlkup; auto.
+    destruct Hlkup; subst. auto.
+  subst.
+  eauto.
+Qed.
+
+Lemma inserted_store__in__phinodes_placement_blk: forall b lid pid sid pds
+  (HeqR1 : ret (lid, pid, sid) = (PI_newids pinfo) ! (getBlockLabel b))
+  (HeqR3 : ret pds = (PI_preds pinfo) ! (getBlockLabel b))
+  (Hneq : pds <> nil) (Hin: blockInFdefB b (PI_f pinfo) = true),
+  insnInFdefBlockB
+     (insn_cmd
+        (insn_store sid (PI_typ pinfo) (value_id pid)
+           (value_id (PI_id pinfo)) (PI_align pinfo)))
+     (phinodes_placement_f pinfo (PI_f pinfo))
+     (phinodes_placement_blk pinfo b) = true.
+Proof.
+  intros.
+  eapply phinodes_placement_blk_head_inv in HeqR1; eauto 1.
+  destruct HeqR1 as [l0 [ps0 [cs0 [tmn0 [cs2 [EQ1 EQ2]]]]]]; subst.
+  apply insnInFdefBlockB_intro.
+    rewrite EQ2.
+    simpl.
+    apply orb_true_intro. left. solve_refl.
+  
+    fold_PhiPlacement_tac.
+    apply TransCFG.pres_blockInFdefB; auto.
+Qed.
+
+Lemma insert_phi__lookupBlockViaIDFromFdef: forall b lid pid sid pds
+  (HeqR1 : ret (lid, pid, sid) = (PI_newids pinfo) ! (getBlockLabel b))
+  (HeqR3 : ret pds = (PI_preds pinfo) ! (getBlockLabel b))
+  (Hneq : pds <> nil) (Hin: blockInFdefB b (PI_f pinfo) = true),
+  lookupBlockViaIDFromFdef (phinodes_placement_f pinfo (PI_f pinfo)) pid =
+    ret (phinodes_placement_blk pinfo b).
+Proof.
+  intros.
+  eapply phinodes_placement_blk_head_inv in HeqR1; eauto 1.
+  destruct HeqR1 as [l0 [ps0 [cs0 [tmn0 [cs2 [EQ1 EQ2]]]]]]; subst.
+  rewrite EQ2.
+  eapply inGetBlockIDs__lookupBlockViaIDFromFdef; eauto 1.
+    rewrite <- phinodes_placement_f_spec1.
+    apply phinodes_placement__uniqFdef; auto.
+
+    simpl. auto.
+  
+    rewrite <- EQ2.
+    fold_PhiPlacement_tac.
+    apply TransCFG.pres_blockInFdefB; auto.
+Qed.
+
+Lemma inserted_phi__wf_value: forall b lid pid sid pds
+  (HeqR1 : ret (lid, pid, sid) = (PI_newids pinfo) ! (getBlockLabel b))
+  (HeqR3 : ret pds = (PI_preds pinfo) ! (getBlockLabel b))
+  (Hneq : pds <> nil) (HBinF: blockInFdefB b (PI_f pinfo) = true),
+  wf_value [M'] M' f' (value_id pid) (PI_typ pinfo).
+Proof.
+  intros. 
+  assert (Hwft:=wf_PI_typ').
+  subst.
+  constructor; auto.
+    eapply phinodes_placement_blk_head_inv in HeqR1; eauto.
+    destruct HeqR1 as [l0 [ps0 [cs0 [tmn0 [cs2 [J3 J4]]]]]]; subst.
+    match goal with
+    | J4: _ = block_intro ?l0 ([?p0]++?ps0) ?cs2 ?tmn |- _ =>
+    apply uniqF__lookupPhiNodeTypViaIDFromFdef with (l1:=l0)
+      (ps1:=[p0]++ps0) (cs1:=cs2)(tmn1:=tmn)(p:=p0); auto
+    end.
+      rewrite <- phinodes_placement_f_spec1.
+      apply phinodes_placement__uniqFdef; auto.
+  
+      rewrite <- J4. 
+      fold_PhiPlacement_tac.
+      apply TransCFG.pres_blockInFdefB; auto.
+  
+      xsolve_in_list.
+Qed.
+
+Lemma wf_operand_phi__in__inserted_store: forall b lid pid sid pds
+  (HeqR1 : ret (lid, pid, sid) = (PI_newids pinfo) ! (getBlockLabel b))
+  (HeqR3 : ret pds = (PI_preds pinfo) ! (getBlockLabel b))
+  (Hneq : pds <> nil) (Hin: blockInFdefB b (PI_f pinfo) = true),
+   wf_operand (phinodes_placement_f pinfo (PI_f pinfo))
+     (phinodes_placement_blk pinfo b)
+     (insn_cmd
+        (insn_store sid (PI_typ pinfo) (value_id pid)
+           (value_id (PI_id pinfo)) (PI_align pinfo))) pid.
+Proof.
+  intros.
+  econstructor; simpl; eauto 2; simpl; auto.
+    eapply inserted_store__in__phinodes_placement_blk; eauto.
+    solve_isNotPhiNode.
+
+    left. 
+    exists (phinodes_placement_blk pinfo b).
+    split.
+      eapply insert_phi__lookupBlockViaIDFromFdef; eauto.
+   
+      destruct (isReachableFromEntry_dec
+                  (phinodes_placement_f pinfo (PI_f pinfo))
+                  (phinodes_placement_blk pinfo b)); auto.
+      left.
+      eapply phinodes_placement_blk_head_inv in HeqR1; eauto 1.
+      destruct HeqR1 as [l1 [ps1 [cs4 [tmn1 [cs5 [EQ1 EQ2]]]]]].
+      subst.
+      rewrite EQ2.
+      simpl.
+      left.
+      match goal with
+      | |- context [?a :: ?B] => 
+           exists nil; exists a; exists B; simpl_env; split; auto
+      end.
+Qed.
+
+Lemma wf_operand_pid__in__inserted_store: forall b lid pid sid pds
+  (HeqR1 : ret (lid, pid, sid) = (PI_newids pinfo) ! (getBlockLabel b))
+  (HeqR3 : ret pds = (PI_preds pinfo) ! (getBlockLabel b))
+  (Hneq : pds <> nil) (Hin: blockInFdefB b (PI_f pinfo) = true),
+  wf_operand (phinodes_placement_f pinfo (PI_f pinfo))
+     (phinodes_placement_blk pinfo b)
+     (insn_cmd
+        (insn_store sid (PI_typ pinfo) (value_id pid)
+           (value_id (PI_id pinfo)) (PI_align pinfo))) (PI_id pinfo).
+Proof.
+  intros.
+  econstructor; simpl; eauto 2; simpl; auto.
+    eapply inserted_store__in__phinodes_placement_blk; eauto.
+    solve_isNotPhiNode.
+
+    left. assert (J:=Hwfpi).
+    apply WF_PhiInfo__lookupBlockViaIDFromFdef in J; auto.
+    destruct J as [be [Hentry Hlkup]]. 
+    apply phinodes_placement_lookupBlockViaIDFromFdef in Hlkup.
+    exists (phinodes_placement_blk pinfo be).
+    split; auto.
+    destruct (isReachableFromEntry_dec
+                (phinodes_placement_f pinfo (PI_f pinfo))
+                (phinodes_placement_blk pinfo b)); auto.
+    destruct (eq_atom_dec (getBlockLabel (phinodes_placement_blk pinfo be))
+                          (getBlockLabel (phinodes_placement_blk pinfo b))).
+    Case "be = b".
+      left.
+      assert (be = b) as EQ.
+        eapply phinodes_placement_blk_rev_eq; eauto.
+      subst.
+      assert (J:=Hwfpi).
+      apply WF_PhiInfo_spec22 in J; auto.
+      destruct J as [l0 [ps0 [cs1 [cs3 [tmn0 Hentry']]]]].
+      uniq_result. simpl in HeqR3.
+      assert (forall pd pds, (PI_preds pinfo) ! l0 <> Some (pd::pds)) as Hprds.
+        intros.
+        eapply PI_preds_of_entry_cannot_be_nonempty in Hentry; eauto 1.
+      rewrite <- HeqR3 in Hprds.
+      destruct pds; congruence.
+
+    Case "be <> b".
+      right. left.
+      fold_PhiPlacement_tac.
+      erewrite <- TransCFG.pres_blockStrictDominates; eauto.
+      assert (isReachableFromEntry (PI_f pinfo) b) as Hreach.
+        erewrite (@TransCFG.pres_isReachableFromEntry (PhiPlacement pinfo)); 
+          eauto.
+      rewrite <- phinodes_placement_blk__getBlockLabel in n.
+      rewrite <- phinodes_placement_blk__getBlockLabel in n.
+      eapply entry_blockStrictDominates_others; eauto.
+Qed.
+
+Lemma inserted_phi__in__phinodes_placement_blk: forall b lid pid sid pds
+  (HeqR1 : ret (lid, pid, sid) = (PI_newids pinfo) ! (getBlockLabel b))
+  (HeqR3 : ret pds = (PI_preds pinfo) ! (getBlockLabel b))
+  (Hneq : pds <> nil) (Hin: blockInFdefB b (PI_f pinfo) = true),
+  insnInFdefBlockB
+     (insn_phinode (gen_phinode pid (PI_typ pinfo) (PI_newids pinfo) pds))
+     (phinodes_placement_f pinfo (PI_f pinfo))
+     (phinodes_placement_blk pinfo b) = true.
+Proof.
+  intros.
+  eapply phinodes_placement_blk_head_inv in HeqR1; eauto 1.
+  destruct HeqR1 as [l0 [ps0 [cs0 [tmn0 [cs2 [EQ1 EQ2]]]]]]; subst.
+  apply insnInFdefBlockB_intro.
+    rewrite EQ2.
+    simpl.
+    apply orb_true_intro. left. solve_refl.
+  
+    fold_PhiPlacement_tac.
+    apply TransCFG.pres_blockInFdefB; auto.
+Qed.
+
+Lemma inserted_phi_operands__elim_aux: forall v l1 pds acc
+  (Hin : In (v, l1)
+          (fold_left
+             (fun (acc : list (value * atom)) (p : atom) =>
+              (match (PI_newids pinfo) ! p with
+               | ret (lid0, _, _) => value_id lid0
+               | merror => value_const (const_undef (PI_typ pinfo))
+               end, p) :: acc) pds acc)),
+  In (v, l1) acc \/ (In l1 pds /\ 
+  match v with
+  | value_id vid1 => 
+      exists pid, exists sid, (PI_newids pinfo) ! l1 = Some (vid1, pid, sid)
+  | value_const vc => vc = const_undef (PI_typ pinfo)
+  end).
+Proof.
+  induction pds as [|a]; simpl; intros; auto.
+    apply IHpds in Hin.
+    destruct Hin as [Hin | [J1 J2]].
+      destruct_in Hin.
+        remember ((PI_newids pinfo) ! a) as R.
+        destruct R as [[[]]|]; inv Hin; right; split; eauto.
+
+      right. split; auto.  
+Qed.
+
+Lemma inserted_phi_operands__elim: forall v l1 pds
+  (Hin : In (v, l1)
+          (fold_left
+             (fun (acc : list (value * atom)) (p : atom) =>
+              (match (PI_newids pinfo) ! p with
+               | ret (lid0, _, _) => value_id lid0
+               | merror => value_const (const_undef (PI_typ pinfo))
+               end, p) :: acc) pds nil)),
+  In l1 pds /\ 
+  match v with
+  | value_id vid1 => 
+      exists pid, exists sid, (PI_newids pinfo) ! l1 = Some (vid1, pid, sid)
+  | value_const vc => vc = const_undef (PI_typ pinfo)
+  end.
+Proof.
+  intros.
+  apply inserted_phi_operands__elim_aux in Hin.
+  destruct Hin as [Hin | Hin]; auto.
+    tauto.
+Qed.
+
+Lemma wf_inserted_phi: forall b lid pid sid pds
+  (HeqR1 : ret (lid, pid, sid) = (PI_newids pinfo) ! (getBlockLabel b))
+  (HeqR3 : ret pds = (PI_preds pinfo) ! (getBlockLabel b)) (Hneq : pds <> nil),
+  wf_phinode (phinodes_placement_f pinfo (PI_f pinfo))
+    (phinodes_placement_blk pinfo b)
+    (gen_phinode pid (PI_typ pinfo) (PI_newids pinfo) pds).
+Proof.
+  intros.
+  constructor.
+    apply wf_phi_operands__intro.
+    intros.
+    apply inserted_phi_operands__elim in Hin.
+    destruct Hin as [Hin [pid' [sid' Hnids]]].
+      assert ((PI_newids pinfo) ! l1 <> merror) as G. congruence.
+      apply PI_newids_are_in_PI_rd in G; auto.
+      apply PI_rd__lookupBlockViaLabelFromFdef in G; auto.
+      destruct G as [b1 [Hlkup Hreach]].
+      assert (Hlkup':=Hlkup).
+      apply (@TransCFG.pres_lookupBlockViaLabelFromFdef (PhiPlacement pinfo)) 
+        in Hlkup'.
+      rewrite (@TransCFG.pres_isReachableFromEntry (PhiPlacement pinfo)) 
+        in Hreach.
+      fold_PhiPlacement_tac.
+      exists (btrans (PhiPlacement pinfo) b1).
+      split; auto.
+      left.
+      exists (btrans (PhiPlacement pinfo) b1).
+      split.
+        apply inGetBlockIDs__lookupBlockViaIDFromFdef; auto.
+          simpl. 
+          rewrite <- phinodes_placement_f_spec1.
+          apply phinodes_placement__uniqFdef; auto.
+
+          eapply WF_PhiInfo_br_preds_succs' in HeqR3; eauto.
+          destruct HeqR3 as [EQ [succs [Hneq' J2]]]; subst.
+          symmetry in Hnids.
+          eapply phinodes_placement_blk_tail_inv in Hnids; eauto.
+          destruct Hnids as [l0 [ps0 [cs0 [tmn0 [ps2 [cs2 [J3 J4]]]]]]]; subst.
+          unfold_PhiPlacement_tac. rewrite J4.
+          simpl. repeat rewrite getCmdsIDs_app. simpl. 
+          xsolve_in_list.
+
+          apply TransCFG.pres_blockInFdefB; auto.
+          solve_blockInFdefB.
+
+        left.
+        apply blockDominates_refl.
+               
+    unfold check_list_value_l.
+    admit. (* 1) redefined predOfBlock by make_pred, or prove they equal.
+              2) br v l1 l2 should ensure l1 <> l2, or ignore the checking *)
+Qed.
+
+Lemma in_map_fst__in_map: forall value_ vls,
+  In value_ 
+    (List.map (fun pat_ : value * l => let (value_0, _) := pat_ in value_0) vls) 
+  ->
+  exists l0, In (value_, l0) vls.
+Proof.
+  induction vls as [|[]]; intros.
+    inv H.
+
+    simpl in H. simpl.
+    inv H; eauto.
+      apply IHvls in H0. 
+      destruct H0 as [l1 H0]. eauto.
+Qed.
+
+Lemma inserted_load__lookupTypViaIDFromFdef: forall (pds : list l) b
+  (HeqR3 : ret pds = (PI_preds pinfo) ! (getBlockLabel b))
+  (vid1 : id) (l0 : l) (Hin : In l0 pds) (pid' : id) (sid' : id)
+  (J : (PI_newids pinfo) ! l0 = ret (vid1, pid', sid')),
+  lookupTypViaIDFromFdef (phinodes_placement_f pinfo (PI_f pinfo)) vid1 =
+    ret PI_typ pinfo.
+Proof.
+  intros.
+  assert ((PI_newids pinfo) ! l0 <> merror) as G. congruence.
+  apply PI_newids_are_in_PI_rd in G; auto.
+  apply PI_rd__lookupBlockViaLabelFromFdef in G; auto.
+  destruct G as [b1 [Hlkup Hreach]].
+  
+  eapply WF_PhiInfo_br_preds_succs' in HeqR3; eauto.
+  destruct HeqR3 as [EQ [succs [Hneq' J1]]]; subst.
+  eapply phinodes_placement_blk_tail_inv in J1; eauto.
+  destruct J1 as [l0 [ps0 [cs0 [tmn0 [ps2 [cs2 [J3 J4]]]]]]]; subst.
+  
+  match goal with
+  | J4: _ = block_intro ?l0 ?ps0 (?cs2 ++ ?cs3 ++ [?c0]) ?tmn |- _ =>
+    apply uniqF__lookupTypViaIDFromFdef with (l1:=l0)(ps1:=ps0)
+      (cs1:=cs2 ++ cs3 ++ [c0])(tmn1:=tmn)(c:=c0); auto
+  end.
+    rewrite <- phinodes_placement_f_spec1.
+    apply phinodes_placement__uniqFdef; auto.
+  
+    rewrite <- J4. 
+    fold_PhiPlacement_tac.
+    apply TransCFG.pres_blockInFdefB; auto.
+    simpl in Hlkup.
+    solve_blockInFdefB.
+  
+    xsolve_in_list.
+Qed.
+
+Lemma inserted_incoming_value__wf_value: forall b lid pid sid pds
+  (HeqR1 : ret (lid, pid, sid) = (PI_newids pinfo) ! (getBlockLabel b))
+  (HeqR3 : ret pds = (PI_preds pinfo) ! (getBlockLabel b)),
+  forall value_ : value,
+  In value_
+     (List.map (fun pat_ : value * l => let (value_0, _) := pat_ in value_0)
+        (fold_left
+           (fun (acc : list (value * atom)) (p : atom) =>
+            (match (PI_newids pinfo) ! p with
+             | ret (lid0, _, _) => value_id lid0
+             | merror => value_const (const_undef (PI_typ pinfo))
+             end, p) :: acc) pds nil)) ->
+  wf_value [M'] M' f' value_ (PI_typ pinfo).
+Proof.
+  intros.
+  apply in_map_fst__in_map in H.
+  destruct H as [l0 Hin].
+  apply inserted_phi_operands__elim in Hin.
+  destruct Hin as [Hin J].
+  assert (wf_typ [M'] (los, nts) (PI_typ pinfo)) as Hwft.
+    apply wf_PI_typ'.
+  destruct value_ as [vid1 | vc1].
+    destruct J as [pid' [sid' J]].
+    subst.
+    constructor; auto.
+      eapply inserted_load__lookupTypViaIDFromFdef; eauto.
+
+    subst.
+    constructor; auto.
+      constructor; auto.
+Qed.
+
+Lemma wf_inserted: forall b b' 
+  (Heqb': b' = phinodes_placement_blk pinfo b)
+  (HBinF: blockInFdefB b (PI_f pinfo) = true),
+  match (PI_newids pinfo) ! (getBlockLabel b) with
+  | Some (lid, pid, sid) =>
+      match (PI_succs pinfo) ! (getBlockLabel b) with
+      | Some (_::_) =>
+          wf_insn [M'] M' f' b' 
+            (insn_cmd (insn_load lid (PI_typ pinfo) (value_id (PI_id pinfo))
+                                 (PI_align pinfo)))
+      | _ => True
+      end /\
+      match (PI_preds pinfo) ! (getBlockLabel b) with
+      | Some ((_::_) as pds) =>
+         wf_insn [M'] M' f' b' 
+           (insn_cmd (insn_store sid (PI_typ pinfo) (value_id pid)
+                        (value_id (PI_id pinfo)) (PI_align pinfo))) /\
+         wf_phinodes [M'] M' f' b' 
+            [gen_phinode pid (PI_typ pinfo) (PI_newids pinfo) pds]
+      | _ => True
+      end
+  | _ => True
+  end.
+Proof.
+  intros. 
+  assert (wf_value [M'] M' f' (value_id (PI_id pinfo)) 
+            (typ_pointer (PI_typ pinfo))) as Hwfv.
+    eapply phinodes_placement_wf_value; eauto.
+      subst. apply WF_PhiInfo__wf_value; auto.
+  assert (wf_typ [M'] (los,nts) (PI_typ pinfo)) as Hwft.
+    apply wf_PI_typ'.
+  remember ((PI_newids pinfo) ! (getBlockLabel b)) as R1.
+  remember ((PI_succs pinfo) ! (getBlockLabel b)) as R2.
+  remember ((PI_preds pinfo) ! (getBlockLabel b)) as R3.
+  destruct R1 as [[[lid pid] sid]|]; auto.
+  split.
+    destruct R2 as [[]|]; auto.
+    assert (l0 :: l1 <> nil) as Hneq. congruence.
+    subst.
+    constructor; auto.
+      eapply wf_insn_base_intro; eauto 1.
+        eapply inserted_load__in__phinodes_placement_blk; eauto.
+
+        simpl. intros id_ Hin.
+        destruct Hin as [Hin | Hin]; subst; try tauto.
+        eapply wf_operand_pid__in__inserted_load; eauto. 
+
+    destruct R3 as [[]|]; auto.
+    assert (l0 :: l1 <> nil) as Hneq. congruence.
+    split.
+      assert (wf_value [M'] M' f' (value_id pid) (PI_typ pinfo)) as Hwfphi.
+        eapply inserted_phi__wf_value; eauto.
+      subst.
+      constructor; auto.
+        eapply wf_insn_base_intro; eauto 1.
+          eapply inserted_store__in__phinodes_placement_blk; eauto. 
+
+          simpl. intros id_ Hin.
+          destruct Hin as [Hin | [Hin | Hin]]; subst; try tauto.
+            eapply wf_operand_phi__in__inserted_store; eauto. 
+            eapply wf_operand_pid__in__inserted_store; eauto. 
+
+      assert (J:=@inserted_incoming_value__wf_value b lid pid sid (l0::l1)
+        HeqR1 HeqR3).
+      subst.
+      constructor; try constructor.
+        auto.
+        eapply inserted_phi__in__phinodes_placement_blk; eauto. 
+        eapply wf_inserted_phi; eauto. 
+Qed.
+
+Lemma phinodes_placement_blockInSystemModuleFdefB: forall b b' 
+  (Heqb': b' = phinodes_placement_blk pinfo b)
+  (Hin: blockInSystemModuleFdefB b [M] M (PI_f pinfo)),
+  blockInSystemModuleFdefB b' [M'] M' f'.
+Proof.
+  intros.
+  subst.
+  apply blockInSystemModuleFdef_inv in Hin.
+  destruct Hin as [J1 [J2 [J3 J4]]].
+  apply blockInSystemModuleFdef_intro.
+    fold_PhiPlacement_tac.
+    apply TransCFG.pres_blockInFdefB; auto.
+
+    apply InProductsB_middle.
+
+    unfold moduleInSystem. simpl.
+    apply orb_true_intro.
+    left. solve_refl.
+Qed.
+
+Lemma phinodes_placement_wf_block : forall b
   (HwfB : wf_block [M] M (PI_f pinfo) b) (Huniq : NoDup (getBlockLocs b))
   (HBinF: blockInFdefB b (PI_f pinfo) = true),
   wf_block [M'] M' f' (phinodes_placement_blk pinfo b).
@@ -408,14 +1613,16 @@ Ltac phinodes_placement_wf_block_tac2 :=
   constructor; try solve [auto | phinodes_placement_wf_block_tac1].
 
   intros.
-  assert (HwfNew:=HwfF).
+  assert (HwfNew:=HBinF).
   eapply wf_inserted in HwfNew; eauto.
-  inv_wf_block HwfB. simpl in HwfNew.
+  inv_wf_block HwfB. 
+
   eapply phinodes_placement_blockInSystemModuleFdefB in HBinSMF; eauto.
   eapply phinodes_placement_wf_cmds in Hwfcs; eauto.
   eapply phinodes_placement_wf_phinodes in Hwfps; eauto.
   eapply phinodes_placement_wf_insn in Hwfi; eauto.
   unfold phinodes_placement_blk, phinodes_placement_block in *.
+  subst b. simpl in HwfNew.
   remember (PI_newids pinfo) ! l5 as R1.
   destruct R1 as [[[lid pid] sid]|]; try solve [constructor; auto].
   remember ((PI_preds pinfo) ! l5) as R2.
@@ -425,21 +1632,17 @@ Ltac phinodes_placement_wf_block_tac2 :=
       try solve [simpl_env in *; phinodes_placement_wf_block_tac2].
 Qed.
 
-Lemma phinodes_placement_wf_blocks : forall (M M':module) (f':fdef)
-  (HwfF: wf_fdef [M] M (PI_f pinfo)) 
-  (HeqM: M = module_intro los nts (Ps1 ++ product_fdef (PI_f pinfo) :: Ps2))
-  (HeqM': M' = module_intro los nts (Ps1 ++ product_fdef f' :: Ps2))
-  (HeqF': f' = phinodes_placement_f pinfo (PI_f pinfo))
-  bs (Hin: forall b, In b bs -> blockInFdefB b (PI_f pinfo) = true)
+Lemma phinodes_placement_wf_blocks : forall bs 
+  (Hin: forall b, In b bs -> blockInFdefB b (PI_f pinfo) = true)
   (HwfBs : wf_blocks [M] M (PI_f pinfo) bs) (Huniq : NoDup (getBlocksLocs bs)),
   wf_blocks [M'] M' f' (List.map (phinodes_placement_blk pinfo) bs).
 Proof.
-  intros. subst.
+  intros. 
   induction bs; simpl.
     constructor.
 
     simpl in Huniq.
-    split_NoDup. inv HwfBs.
+    split_NoDup. inversion HwfBs.
     constructor; auto.
       eapply phinodes_placement_wf_block; eauto 1.
         apply Hin; simpl; auto.
@@ -447,19 +1650,11 @@ Proof.
         intros b Hin'. apply Hin. simpl; auto.
 Qed.
 
-Lemma In_InBlocksB: forall b bs, In b bs -> InBlocksB b bs = true.
-Admitted.
-
-Lemma phinodes_placement_wf_fdef: forall (M M':module) (f':fdef)
-  (HeqM: M = module_intro los nts (Ps1 ++ product_fdef (PI_f pinfo) :: Ps2))
-  (HeqM': M' = module_intro los nts (Ps1 ++ product_fdef f' :: Ps2))
-  (HeqF': f' = phinodes_placement_f pinfo (PI_f pinfo))
-  f (HwfF: wf_fdef [M] M f) 
-  (Heq: f = PI_f pinfo) (HuniqF: uniqFdef f), 
+Lemma phinodes_placement_wf_fdef: 
   wf_fdef [M'] M' (phinodes_placement_f pinfo (PI_f pinfo)).
 Proof.
-  intros. subst. assert (HwfF':=HwfF).
-  inv HwfF'.
+  intros. assert (HwfF':=HwfF).
+  inv_wf_fdef HwfF'.
   match goal with
   | Hentry : getEntryBlock _ = _,
     HuniqF : uniqFdef _,
@@ -470,6 +1665,19 @@ Proof.
      eapply (@TransCFG.pres_hasNonePredecessor (PhiPlacement pinfo)) 
        in Hnpred; eauto
   end.
+  rewrite EQ2 in Hwfb.
+  match goal with
+  | H2: fdef_intro _ _ = PI_f _,
+    H9: wf_blocks _ _ _ _ |- _ =>
+    rewrite H2 in H9;
+    eapply phinodes_placement_wf_blocks in H9; try solve [
+      eauto |
+      rewrite <- H2 in HuniqF; eapply uniqF__uniqBlocksLocs; eauto |
+      rewrite <- H2; simpl; intros; apply In_InBlocksB; auto
+    ]
+  end.
+
+  subst. uniq_result. rewrite <- EQ3.
   eapply wf_fdef_intro; eauto 2.
     clear. 
     apply productInSystemModuleB_intro.
@@ -485,17 +1693,10 @@ Proof.
       intros t0 Hint0.
       apply H0 in Hint0.
       eapply wf_typ_independent; eauto.
-
+  
     match goal with
-    | H2: fdef_intro _ _ = PI_f _,
-      H9: wf_blocks _ _ _ _ |- _ =>
-      rewrite H2 in H9;
-      eapply phinodes_placement_wf_blocks in H9; try solve [
-        eauto |
-        rewrite <- H2; fold_PhiPlacement_tac |
-        rewrite <- H2 in HuniqF; eapply uniqF__uniqBlocksLocs; eauto |
-        rewrite <- H2; simpl; intros; apply In_InBlocksB; auto
-      ]
+    | H2: fdef_intro _ _ = PI_f _, H9: wf_blocks _ _ _ _ |- _ =>
+      rewrite <- H2 in H9; auto
     end.
 Qed.
     
